\documentclass[12pt]{article}

\usepackage{sbc-template}
\usepackage{graphicx,url}
%\usepackage[brazil]{babel}
\usepackage[latin1]{inputenc}  
\usepackage{amsmath, amsthm, amssymb}
\usepackage{enumitem}
\usepackage{proof}
\usepackage{coqdoc}
\usepackage{listings,lstlangcoq,bold-extra}
\lstset{basicstyle=\ttfamily,language=Coq,showstringspaces=false}
     
\sloppy

\title{A Semantical Proof of Consistency for Minimal Propositional Logic in Coq}

\author{Felipe Sasdelli\inst{1}, Maycon Amaro\inst{1}, Rodrigo Ribeiro\inst{1}}


\address{Departamento de Computa\c{c}\~ao -- Universidade Federal de Ouro Preto
  (UFOP)\\
  35400-000 -- Ouro Preto -- MG -- Brazil
  \email{\{felipe.sasdelli,maycon.amaro\}@aluno.ufop.edu.br,
    rodrigo.ribeiro@ufop.edu.br}
}

\theoremstyle{definition}
\newtheorem{Theorem}{Theorem}
\newtheorem{Corollary}{Corollary}
\newtheorem{Lemma}{Lemma}

\newlist{Cases}{enumerate}{4}
\setlist[Cases]{align=left,
                 listparindent=\parindent, 
                 parsep=\parskip, 
                 font=\normalfont\bfseries, 
                 leftmargin=0pt,
                 labelwidth=0pt, 
                 itemindent=.4em,labelsep=.4em,
                 partopsep=0pt
                 }

\setlist[Cases,1]{label=Case~\arabic*:,ref=\arabic*}
\setlist[Cases,2]{label=Case~\theCasesi.\roman*:,ref=\theCasespi.\roman*}
\setlist[Cases,3]{label=Case~\theCasesii.\alph*:,ref=\theCasespii.\alph*}

                 
\begin{document} 

\maketitle

\begin{abstract}
  Consistency is a key property of any logical system. However, proofs of
  consistency usually rely on heavy proof theory notions like admissibility
  of cut. A more semantics-based approach to consistency proofs is to explore the
  correspondence between a logics and its relation with the
  evaluation in a $\lambda$-calculus, known as Curry-Howard isomorphism.
  In this work, we describe a Coq formalization of consistency of minimal
  propositional logics using this semantics approach and compare it with 
  the traditional ones used in proof theory.
\end{abstract}

\input{consistency.tex}

\bibliographystyle{sbc}
\bibliography{template}

\appendix

\section{Consistency Proof Based on Admissibility}

\subsection{Overview}

Due to limited space, we include a brief description of our formalization of
consistency using Gentzen's cut-elimination method in this appendix. First, we
present types for describing the syntax of formulas, natural deduction
and sequent calculus proofs. Next, we provide proof sketchs of the main
properties proved to ensure consistency of the minimal logic considered.

\subsection{Basic Definitions}

Unlike in our semantics based proof, we need to represent variables in
formula syntax. We chose to represent variable identifiers as natural
numbers.

\begin{lstlisting}
Definition var := nat.

Inductive form : Type :=
| Falsum  : form 
| Var     : var -> form
| Implies : form -> form -> form.
\end{lstlisting}

Constructors \lstinline{Falsum} e \lstinline{Implies} represent the
false constant and logical implication, respectively. Using the defined
syntax, we can represent natural deduction and sequent calculus rules as
inductive types as presented next.

\begin{minipage}[c]{0.6\textwidth}
\begin{lstlisting}
Inductive nd : ctx -> form -> Prop :=
| Id_Nd G a
  : a el G ->
    nd G a
| ExFalsum G a
  : nd G Falsum ->
    nd G a
| Implies_I G a b
  : nd (a :: G) b ->
    nd G (Implies a b)
| Implies_E G a b
  : nd G (Implies a b) ->
    nd G a -> nd G b.
\end{lstlisting}
\end{minipage}
\begin{minipage}[c]{0.3\textwidth}
\[
\begin{array}{c}
\infer[_{\{Id\}}]{\Gamma \vdash x}{x \in \Gamma} \\ \\
\infer[_{\{Ex\}}]{\Gamma \vdash \alpha}{\Gamma \vdash \bot}\\ \\
\infer[_{\{\supset-I\}}]{\Gamma \vdash \alpha \supset \beta}{\Gamma \cup \{\alpha\} \vdash \beta}\\ \\
\infer[_{\{\supset-E\}}]{\Gamma \vdash \beta}{\Gamma \vdash \alpha \supset \beta & \Gamma \vdash \alpha}
\end{array}
\]
\end{minipage}

The only change on how we represent the natural deduction proof system is in the
rule for variables. We use the Coq library boolean list membership predicate
(\lstinline{member}), which fits better for proof automation. In order to
simplify the task of writing code that uses this predicate, we defined
notation \lstinline{a el G} which means \lstinline{member a G}. The other
constructors of type \lstinline{nd} are identitical to the ones presented in
Section~\ref{sec:semantics}.

Next, we the sequent calculus formulation for our minimal logic. The only
difference with the natural deduction is in one rule for implication. The
sequent calculus rule counter-part for implication elimination is called
implication left rule, which states that we can conclude any formula $\gamma$
in a context $\Gamma$ if we have that: 1) $\alpha \supset \beta \in \Gamma$;
2) $\Gamma \Rightarrow \alpha$ and 3) $\Gamma \cup \{\beta\} \Rightarrow
\gamma$. The rules for the sequent-calculus and its correspondent Coq
implementation are presented next.

\begin{minipage}[c]{0.6\textwidth}
\begin{lstlisting}
Inductive sc : ctx -> form -> Prop :=
| Id G a
  : (Var a) el G ->
    sc G (Var a)
| Falsum_L G a
  : Falsum el G ->
    sc G a
| Implies_R G a b
  : sc (a :: G) b ->
    sc G (Implies a b)
| Implies_L G a b c
  : (Implies a b) el G ->
    sc G a ->
    sc (b :: G) c ->
    sc G c.  
\end{lstlisting}
\end{minipage}
\begin{minipage}[c]{0.3\textwidth}
\[
\begin{array}{c}
\infer[_{\{Id\}}]{\Gamma \Rightarrow x}{x \in \Gamma} \\ \\
\infer[_{\{Ex\}}]{\Gamma \Rightarrow \alpha}{\Gamma \Rightarrow \bot}\\ \\
\infer[_{\{\supset-R\}}]{\Gamma \Rightarrow \alpha \supset \beta}{\Gamma \cup \{\alpha\} \Rightarrow \beta}\\ \\
  \infer[_{\{\supset-L\}}]{\Gamma \Rightarrow \gamma}{\begin{array}{c}
                                                       \alpha \supset \beta \in
                                                        \Gamma \\
                                                        \Gamma \Rightarrow
                                                        \alpha \\ \Gamma \cup
                                                        \{\beta\}\vdash \gamma
                                                    \end{array}}
\end{array}
\]
\end{minipage}

Using the previous definitions we can prove consistency of our minimal logic by
implementing Gentzen's argument using Coq. In the next section, we outline the
theorems and lemmas proved.

\section{Proving Consistency}

In order to prove the admissibility of cut for sequent-calculus, we need to
prove \emph{weakening}, which states that the inclusion of new hypothesis does
not change provability.

\begin{Lemma}[Weakening]\label{lemma:weak}
  If $\Gamma \Rightarrow \alpha$ and $\Gamma \subseteq \Gamma'$ then $\Gamma'
  \Rightarrow \alpha$.
\end{Lemma}
\begin{proof}
  By structural induction on the derivation of $\Gamma \Rightarrow \alpha$.
  \begin{Cases}
    \item Last rule in the derivation of $\Gamma \Rightarrow \alpha$ was $Id$: In this
    situation, we have that $\alpha \in \Gamma$. Since $\Gamma \subseteq
    \Gamma'$, we have that $\alpha \in \Gamma'$ and the conclusion follows by
    rule $Id$.
    \item Last rule in the derivation of $\Gamma \Rightarrow \alpha$ was $Ex$: In this 
    case, we have that $\Gamma \Rightarrow \bot$. By the induction hypothesis on 
    $\Gamma \Rightarrow \bot$ we have that $\Gamma' \Rightarrow \bot$ and the 
    conclusion follows by rule $Ex$.
    \item Last rule in the derivation of $\Gamma \Rightarrow \alpha$ was $\supset-R$:
    In this situation, we have that $\Gamma \cup \{\alpha\} \Rightarrow \beta$.
    Since we have that $\Gamma \subseteq \Gamma'$, it follows that
    $\Gamma \cup \{\alpha\} \subseteq \Gamma' \cup \{\alpha\}$. By the induction
    hypothesis on $\Gamma \cup \{\alpha\} \Rightarrow \beta$, we have that
    $\Gamma' \cup \{\alpha\} \Rightarrow \beta$ and conclusion follows by rule
    $\supset-R$.
    \item Last rule in the derivation of $\Gamma \Rightarrow \alpha$ was $\supset-L$:
    In this situation, we have that: 1) there exists $\gamma \supset \beta \in
    \Gamma$; 2) $\Gamma \Rightarrow \gamma$ and 3) 
    $\Gamma \cup \{\beta\} \Rightarrow \alpha$. Since, $\gamma \supset
    \beta \in \Gamma$ and $\Gamma \subseteq \Gamma'$, we have that
    $\gamma\supset \beta \in \Gamma'$. Also, we have that
    $\Gamma' \Rightarrow \gamma$ and $\Gamma' \cup \{\beta\}\Rightarrow \alpha$
    by the induction hypothesis on $\Gamma\Rightarrow \gamma$ and
    $\Gamma \cup \{\beta\} \Rightarrow \alpha$, respectively. Conclusion follows
    by rule $\supset-L$.
  \end{Cases}
\end{proof}

Using weakening property we can prove a generalized version of admissibility of
cut. We first prove this auxiliar lemma in order to get a stronger induction
hypothesis. From the next lemma, admissibility is just a corollary.

\begin{Lemma}[Genealized admissibility]\label{lemma:admissibility}
  If $\Gamma \Rightarrow \alpha$ and $\Gamma' \Rightarrow \beta$ then $\Gamma
  \cup (\Gamma' - \{\alpha\}) \Rightarrow \beta$.
\end{Lemma}
\begin{proof}
  By structural induction on $\alpha$.
  \begin{Cases}
     \item $\alpha = \bot$: Now, we proceed by induction on
       $D : \Gamma \Rightarrow \bot$.
    \begin{Cases}
      \item Last rule used in deriving $\Gamma \Rightarrow \bot$ was Id: In this
            situation, we have a contradiction (Var n = Falsum), and the desired
            result follows.
      \item Last rule used in deriving $\Gamma \Rightarrow \bot$ was Ex: We have that
            $\bot \in \Gamma$ and $\Gamma' \Rightarrow \beta$. Conclusion follows by
            rule $Ex$ and the fact that $\bot \in (\Gamma \cup (\Gamma' -
            \{\bot\}))$.
      \item Last rule used in deriving $\Gamma\Rightarrow \bot$ was $\supset-R$:
            In this case we have a contradiction (Implies a b = Falsum), and the
            desired result follows.
      \item Last rule used in deriving $\Gamma\Rightarrow \bot$ was $\supset-L$:
            In this case we have that: 1) $A \supset B \in \Gamma$; 2)
            $\Gamma \Rightarrow A$ and 3) $\Gamma' \cup \{B\} \Rightarrow \bot$. By
            weakening on $\Gamma \Rightarrow A$ we have that
            $\Gamma \cup (\Gamma' -\{B\})\Rightarrow A$. By the induction hypothesis
            of derivation $D$, we have that
            $\Gamma \cup \{B\} \cup (\Gamma' - \{\bot\}) \Rightarrow \beta$ and
            conclusion follows by rule $\supset-L$.
    \end{Cases}
    \item $\alpha = (Var\:v)$: Now we proceed by induction on
      $D : \Gamma \Rightarrow Var\:v$.
      \begin{Cases}
         \item Last rule used in deriving $\Gamma \Rightarrow (Var\:v)$ was Id:
           In this situation, we have that $(Var\:v) \in \Gamma$. Since
           $(Var\:v) \in \Gamma$, we have that $(Var\:v) \in \Gamma \cup (\Gamma'
           - \{Var\:v\})$ and conclusion follows by rule Id.
         \item Last rule used in deriving $\Gamma\Rightarrow (Var\:v)$ was Ex:
           In this situation, we have that $\bot \in \Gamma$. Since $\bot \in
           \Gamma$, we have $\bot \in \Gamma \cup (\Gamma' - \{Var\:v\})$ and
           conclusion follows by rule Ex.
         \item Last rule used in deriving $\Gamma\Rightarrow (Var\:v)$ was
           $\supset-R$: In this situation, we have a contradiction, since
           $Var\:v\neq a \supset b$, for some $a$ and $b$.
         \item Last rule used in deriving $\Gamma\Rightarrow (Var\:v)$ was
           $\supset-L$: In this situation, there exists $a, b$ such that
           $a \supset b \in \Gamma$, $\Gamma \Rightarrow a$ and
           $\Gamma \cup \{b\} \Rightarrow (Var\:v)$. By weakening on
           $\Gamma \Rightarrow a$, we have
           $(\Gamma \cup \{b\})\cup(\Gamma' - \{Var\:v\}) \Rightarrow a$.
           By the induction hypothesis on $\Gamma \cup \{b\} \Rightarrow
           (Var\:v)$, we have
           $\Gamma \cup \{b\} \Rightarrow (Var\:v) \Rightarrow b$.
           Conclusion follows by rule $\supset-L$.
      \end{Cases}
    \item $\alpha = a_1 \supset a_2$: Now, we proceed by induction on
      $D : \Gamma \Rightarrow (a_1 \supset a_2)$.
      \begin{Cases}
        \item Last rule used in deriving $\Gamma \Rightarrow (a_1 \supset a_2)$ was
          Id: This case is a contradiction, since it is not possible that
          $Var\:v = a_1\supset a_2$.
        \item Last rule used in deriving $\Gamma \Rightarrow (a_1 \supset a_2)$ was
          Ex: In this case, we have that $\bot \in \Gamma$. Since
          $\bot \in \Gamma$, we have that
          $\bot \in \Gamma \cup (\Gamma' - \{a_1 \supset a_2\})$ and conclusion
          follows by rule Ex.
        \item Last rule used in deriving $\Gamma \Rightarrow (a_1 \supset a_2)$ was
          $\supset-R$: Now we proceed by induction on $\Gamma' \Rightarrow
          \beta$.
          \begin{Cases}
             \item Last rule used in deriving $\Gamma' \Rightarrow \beta$ was Id:
               In this case, we have that $\beta = Var\:v$ and $Var\:v\in\Gamma'$.
               Since $Var\:v \neq a_1\supset a_2$, we have that
               $Var\:v\in\Gamma \cup (\Gamma' - \{a_1 \supset a_2\})$ and
               conclusion follows by rule Id.
             \item Last rule used in deriving $\Gamma' \Rightarrow \beta$ was
               Ex: In this case, we have that $\bot \in \Gamma'$. Since
               $\bot \neq a_1 \supset a_2$, we have that
               $\bot\in\Gamma \cup (\Gamma' - \{a_1 \supset a_2\})$ and
               conclusion follows by rule Ex.
             \item Last rule used in deriving $\Gamma' \Rightarrow \beta$ was
               $\supset-R$: In this case, $\beta = a \supset b$, for some $a,b$.
               Also, we have that $\Gamma' \cup \{a\}\Rightarrow b$. By the
               induction hypothesis on $\Gamma' \cup \{a\}\Rightarrow b$, we
               have that
               $\Gamma \cup ((\Gamma' \cup \{a\}) - \{a_1 \supset
               a_2\})\Rightarrow b$. Since we have 
               $\Gamma \cup ((\Gamma' \cup \{a\}) - \{a_1 \supset
               a_2\})\Rightarrow b$ then we also have
               $\Gamma \cup (\Gamma' \cup \{a\} - \{a_1 \supset
               a_2\}) \cup \{a\} \Rightarrow b$ and conclusion follows by rule
               $\supset-R$.
             \item Last rule used in deriving $\Gamma' \Rightarrow \beta$ was
               $\supset-L$: In this situation, we have that
               $a \supset b \in \Gamma'$, $\Gamma' \Rightarrow a$ and
               $\Gamma' \cup \{b\} \Rightarrow \beta$. Let's consider that
               $a \supset b = a_1 \supset a_2$. Now, we can deduce
               $\Gamma \cup \Gamma' - \{a_1 \supset a_2\} \Rightarrow a_2$ by
               the induction hypothesis on $\Gamma \cup \{a_1\} \Rightarrow a_2$
               and weakening. Conclusion follows from weakening and
               $\Gamma \cup \Gamma' - \{a_1 \supset a_2\} \Rightarrow a_2$.
               Now, suppose that $a \supset b \neq a_1 \supset a_2$. Conclusion
               follows by the weakening the induction hypothesis on
               $\Gamma' \Rightarrow \beta$ and rule $\sup-L$.
             \end{Cases}
            \item Last rule used in deriving $\Gamma \Rightarrow (a_1 \supset a_2)$ was
              $\supset-L$: By weakening on $\Gamma \Rightarrow a_1$ we have
              $\Gamma \cup (\Gamma' 0 \{a_1 \supset a_2\}) \Rightarrow a_1$.
              Conclusion follows from the induction hypothesis and rule $\supset-L$.
          \end{Cases} 
  \end{Cases}
\end{proof}

\begin{Corollary}[Admissibility of cut]
  If $\Gamma \Rightarrow \alpha$ and $\Gamma \cup\{\alpha\}\Rightarrow \beta$
  then $\Gamma \Rightarrow \beta$.
\end{Corollary}
\begin{proof}
  Immediate consequence of Lemmas~\ref{lemma:weak} and~\ref{lemma:admissibility}.
\end{proof}

Consistency of sequent calculus trivially follows by inspection on the structure of
derivations.

\begin{Theorem}[Consistency of sequent calculus]\label{theorem:consistency}
  There is no proof of $\emptyset \Rightarrow \bot$.
\end{Theorem}
\begin{proof}
  Immediate from the sequent calculus rules (there is no rule to introduce $\bot$).
\end{proof}

The Coq code for all these proofs can be found in file
\href{https://github.com/rodrigogribeiro/consistency-coq/blob/master/Minimal/SequentCalculus.v}{SequentCalculus.v}
on-line~\cite{Sasdelli20}.

The next step in the mechanization of the
consistency of our minimal logic is to stabilish the equivalence between sequent
calculus and natural deduction systems. The equivalence proofs between these two
formalism are based on a routine induction on derivations using admissibility of
cut. We omit its description for brevity. The complete proofs of these
equivalence results can be found in file
\href{https://github.com/rodrigogribeiro/consistency-coq/blob/master/Minimal/NatDed.v}{NatDed.v} in the source code
repository~\cite{Sasdelli20}.

Finally, we can prove the consistency of natural deduction by combining the
proofs of consistency of the sequent calculus and the equivalence between these
formalisms.

\begin{Theorem}[Consistency for Natural Deduction]
  There is no proof of $\emptyset \vdash \bot$.
\end{Theorem}
\begin{proof}
  Suppose that $\emptyset \vdash \bot$. By the equivalence between natural
  deduction and sequent calculus, we have $\emptyset\Rightarrow \bot$, which
  contradicts Theorem~\ref{theorem:consistency}.
\end{proof}  

\end{document}

